dataplane/Operators_Utils.thy
@@ -2,6 +2,7 @@ theory Operators_Utils
 
 imports
   Nondeterministic_Dataflow.Operator
+  Utils
 begin 
 
 corec writes where
@@ -48,6 +49,16 @@ lemma step_writes_silent_buf_empty:
   apply (auto split: op.splits list.splits)
   done
 
+lemma step_writes_elim:
+  assumes "step io (writes op p xs) op'"
+  obtains x xs' where "io = Out p x" "xs = x # xs'" "op' = writes op p xs'"
+  | "xs = []" "step io op op'"
+  using assms apply atomize_elim
+  apply (subst (asm) writes.code)
+  apply (auto split: op.splits list.splits)
+  done
+
+
 lemma step_writes_Out_intro[intro]:
   "buf = x # buf' \<Longrightarrow>
    op' = writes op p buf'\<Longrightarrow>
@@ -88,5 +99,743 @@ lemma writes_Cons_simp:
   apply (subst (asm) writes.code, simp add: op.cong_refl writes.friend.code rel_fun_def split: op.splits)
   apply (subst (asm) writes.code, simp add: op.cong_refl writes.friend.code rel_fun_def split: op.splits)
   done
+
+
+fun steps where
+  "steps [] = (=)"
+| "steps (io # ios) = step io OO steps ios"
+
+lemma steps_append[simp]:
+  "steps (xs @ ys) = steps xs OO steps ys"
+  by (induct xs arbitrary: ys) auto
+
+lemma step_refl[simp]:
+  "step io OO (=) = step io"
+  by auto
+
+thm step_map_op[no_vars]
+
+lemma steps_map_op[intro!]:
+  "op'' = map_op f g op' \<Longrightarrow> 
+   map (map_IO f g id) xs = xs' \<Longrightarrow>
+   steps xs op op' \<Longrightarrow>
+   steps xs' (map_op f g op) op''"
+  by (induct xs' arbitrary: op op' op'' xs)
+    (force simp add: relcompp_apply)+
+
+lemma steps_intro[intro]:
+  "step x op op' \<Longrightarrow>
+   steps xs op' op'' \<Longrightarrow>
+   ys = x # xs \<Longrightarrow>
+   steps ys op op''"
+  apply auto
+  done
+
+lemma steps_intro_alt[intro]:
+  "steps xs op op' \<Longrightarrow>
+   step x op' op'' \<Longrightarrow>
+   ys = xs @ [x] \<Longrightarrow>
+   steps ys op op''"
+  apply auto
+  done
+
+lemma steps_append_intro[intro]:
+  "steps xs op op' \<Longrightarrow>
+   steps ys op' op'' \<Longrightarrow>
+   zs = xs @ ys \<Longrightarrow>
+   steps zs op op''"
+  apply auto
+  done
+
+definition sim_set (\<open>_ \<leadsto>[_] _\<close> [80, 80, 80] 80)
+where
+  "P \<leadsto>[Rel] Q \<equiv> \<forall>io Q'. step io Q Q' \<longrightarrow> (\<exists>P'. step io P P' \<and> (P', Q') \<in> Rel)"
+
+definition wsim_set (\<open>_ \<leadsto>\<^sup>^<_> _\<close> [80, 80, 80] 80)
+where
+  "P \<leadsto>\<^sup>^<Rel> Q \<equiv> \<forall>io Q'. step io Q Q' \<longrightarrow> (\<exists>P'. wstep io P P' \<and> (P', Q') \<in> Rel)"
+
+lemma rel2_in_rel[simp]:
+  "in_rel = rel2p"
+  unfolding rel2p_def by force
+
+lemma in_p2_rel_simp[simp]:
+  "(op1, op2) \<in> p2rel X \<longleftrightarrow> X op1 op2"
+  by (metis case_prodI mem_Collect_eq p2relD p2rel_def)
+
+lemma wsim_set_wsim:
+  "P \<leadsto>\<^sup>^<p2rel R> Q \<longleftrightarrow> wsim (conversep R) Q P"
+  unfolding wsim_def wsim_set_def
+  apply auto
+  done
+
+lemma sim_set_sim:
+  "P \<leadsto>[p2rel R] Q \<longleftrightarrow> sim (conversep R) Q P"
+  unfolding sim_def sim_set_def
+  apply auto
+  done
+
+lemma bisim_converse[simp]:
+  "(~)\<inverse>\<inverse> = (~)"
+  using bisim_sym by blast
+
+lemma wbisim_converse[simp]:
+  "(\<approx>)\<inverse>\<inverse> = (\<approx>)"
+  using wbisim_sym by blast
+
+lemma p2rel_relcompp:
+  "p2rel (R1 OO R2) = p2rel R1 O p2rel R2"
+  by force
+
+
+lemma wsim_set_wsim_ex:
+  "P \<leadsto>\<^sup>^<((p2rel (\<approx>)) O (p2rel X) O (p2rel (~)))> Q \<longleftrightarrow> wsim ((~) OO (conversep X) OO (\<approx>)) Q P"
+  using wsim_set_wsim[where P=P and Q=Q and R="(\<approx>) OO X OO (~)", simplified]
+  by (simp add: p2rel_relcompp relcompp_assoc converse_relcompp)
+
+lemma strongAppend:
+  assumes PSimQ: "P \<leadsto>\<^sup>^<Rel> Q"
+  and     QSimR: "Q \<leadsto>[Rel'] R"
+  and     Trans: "Rel O Rel' \<subseteq> Rel''"
+  shows "P \<leadsto>\<^sup>^<Rel''> R"
+ using assms
+  unfolding wsim_set_def sim_set_def
+  apply blast
+  done
+
+lemma weakSimE:
+  assumes "P \<leadsto>\<^sup>^<Rel> Q"
+  and     "step io Q Q'"
+
+  obtains P' where "wstep io P P'" and "(P', Q') \<in> Rel"
+  using assms apply -
+  apply atomize_elim
+  apply (auto simp add: wsim_set_def)
+  done
+
+lemma weakSimI[case_names Sim]:
+  assumes "\<And>io Q'. step io Q Q' \<Longrightarrow> \<exists>P'. wstep io P P' \<and> (P', Q') \<in> Rel"
+
+  shows "P \<leadsto>\<^sup>^<Rel> Q"
+using assms
+  by(auto simp add: wsim_set_def)
+
+term "p2rel (wbisim_cong X)"
+
+lemma weakBisimWeakCoinduct[consumes 1, case_names cSim cSym]:
+  assumes "(P, Q) \<in> X"
+    and     "\<And>P Q. (P, Q) \<in> X \<Longrightarrow> P \<leadsto>\<^sup>^<X> Q"
+    and     "\<And>P Q. (P, Q) \<in> X \<Longrightarrow> Q \<leadsto>\<^sup>^<X> P"
+  shows "P \<approx> Q"
+  using assms apply -
+  apply (rule wbisim_coinduct_upto)
+   apply assumption
+  apply (intro conjI)
+  apply (metis (mono_tags, lifting) conversep_wbc predicate2I rel2pD rel2p_inv(2) rev_predicate2D wbisim_cong.intros(1) wsim_conversep_mono wsim_set_wsim)+
+  done
+
+lemma
+  "(\<And>R S. (R, S) \<in> Rel \<Longrightarrow> R \<leadsto>\<^sup>^<Rel> S) \<Longrightarrow>
+   (\<And>R S. (R, S) \<in> (converse Rel) \<Longrightarrow> R \<leadsto>\<^sup>^<converse Rel> S)"
+  apply (auto simp add: wsim_set_def wstep_def)
+  oops
+
+
+lemma
+  "(\<And>R S. (R, S) \<in> Rel \<Longrightarrow> R \<leadsto>\<^sup>^<Rel> S) \<Longrightarrow> wbisimulation (rel2p Rel)"
+  apply (auto simp add: wsim_def wsim_set_def rel2p_def)
+  oops
+
+lemma rel2p_converse_simp:
+  "rel2p (Rel\<inverse>) = conversep (rel2p Rel)"
+  unfolding rel2p_def by force
+
+lemma wbisim_wstep_Tau_stronger:
+  assumes "wsimulation_canonical R"
+    and "R op1 op2"
+    and "(step Tau)\<^sup>*\<^sup>* op1 op1'"
+  shows "\<exists>op2'. wstep Tau op2 op2' \<and> R op1' op2'"
+  using assms(3,2)
+proof (induct op1 arbitrary: op2 rule: converse_rtranclp_induct)
+  case (step op1 op1'')
+  with assms(1) obtain op2'' where "wstep Tau op2 op2''" "R op1'' op2''"
+    unfolding wsim_def by (metis wsimulation_canonical_def)
+  moreover from step(3)[OF \<open>R op1'' op2''\<close>] obtain op2' where "wstep Tau op2'' op2'" "R op1' op2'"
+    by blast
+  ultimately show ?case by (auto intro!: exI[of _ op2'])
+qed force
+
+lemma wbisim_wstep_stronger:
+  assumes "wsimulation_canonical R"
+    and "R op1 op2"
+    and "wstep io op1 op1'"
+  obtains op2' where "wstep io op2 op2'" and "R op1' op2'"
+proof -
+  from assms(3) obtain opi opj where \<open>(step Tau)\<^sup>*\<^sup>* op1 opi\<close> \<open>estep io opi opj\<close> \<open>(step Tau)\<^sup>*\<^sup>* opj op1'\<close> unfolding wstep_def by blast
+  moreover from assms(1,2) obtain \<open>wsim R op1 op2\<close> unfolding wsim_def by (simp add: that wsim_correct)
+  ultimately have \<open>\<exists>op2'. wstep io op2 op2' \<and> R op1' op2'\<close> using assms(2)
+  proof (induct op1 arbitrary: op2 rule: converse_rtranclp_induct)
+    case base
+    show ?case
+    proof (cases "io = Tau \<and> opi = opj")
+      case True
+      with base(2,3,4) show ?thesis
+        using wbisim_wstep_Tau_stronger[OF assms(1), of opi op2 op1'] by auto
+    next
+      case False
+      with base obtain opj' where H1: \<open>wstep io op2 opj'\<close> \<open>R opj opj'\<close> unfolding wsim_def by (cases io) force+
+      with assms(1) have \<open>wsim R opj opj'\<close> unfolding wsim_def by (simp add: wsimulation_canonical_def)
+      with base(2) H1(2) have \<open>\<exists>op2'. (step Tau)\<^sup>*\<^sup>* opj' op2' \<and> R op1' op2'\<close>
+        using wbisim_wstep_Tau_stronger[OF assms(1), of opj opj' op1'] by auto
+      with \<open>wstep io op2 opj'\<close> show ?thesis unfolding wstep_def
+        by (smt (verit, best) relcompp_apply rtranclp_trans)
+    qed
+  next
+    case (step op1 opk)
+    from step(1) obtain opk' where "(step Tau)\<^sup>*\<^sup>* op2 opk'" "R opk opk'"
+      by (auto dest!: step(6)[unfolded wsim_def, rule_format])
+    with step(3)[of opk'] step(4,5) assms(1) show ?case unfolding wstep_def
+      by (smt (verit, ccfv_SIG) estep.elims transitive_closurep_trans'(2) wsim_correct wstep_def wstep_steps_Tau wstep_trans'(1,2))
+  qed
+  then show ?thesis using that by force
+qed
+
+
+lemma wsimTransitive:
+  assumes "(P, Q) \<in> Rel"
+  and     "Q \<leadsto>\<^sup>^<Rel'> R"
+  and     "Rel O Rel' \<subseteq> Rel''"
+  and     "\<And>S T. (S, T) \<in> Rel \<Longrightarrow> S \<leadsto>\<^sup>^<Rel> T"
+  shows "P \<leadsto>\<^sup>^<Rel''> R"
+proof(induct rule: weakSimI)
+  case(Sim io R')
+  thus ?case using assms
+    apply(drule_tac Q=R in weakSimE, auto)
+    subgoal for Q'
+      apply (rule wbisim_wstep_stronger[rotated, of "rel2p (converse Rel)" Q P io Q', unfolded rel2p_def, simplified])
+         apply assumption+
+       apply blast
+      apply (auto simp add: wsim_set_def  wsimulation_canonical_def wstep_def wsim_def)
+      done
+    done
+qed
+
+lemma p2rel_converse[simp]:
+  "(p2rel R)\<inverse> = p2rel (conversep R)"
+  by auto
+
+lemma wsim_set_wbisim_l:
+  assumes "P' \<leadsto>\<^sup>^<(p2rel (\<approx>) O X)> Q" 
+    and p: "P \<approx> P'" 
+  shows "P \<leadsto>\<^sup>^<(p2rel (\<approx>) O X)> Q"
+proof -
+  let ?Y = "p2rel (\<approx>) O X"
+  show ?thesis
+  proof -
+    have "(p2rel (\<approx>)) O ?Y \<subseteq> ?Y" using wbisim_trans by fastforce
+    then show ?thesis 
+      using assms apply -
+      apply (rule wsimTransitive)
+         prefer 3
+         apply assumption
+        apply simp_all
+      apply (metis wbisim.cases wbisim_converse wsim_set_wsim)+
+      done
+  qed
+qed
+
+lemma sim_set_bisim_r:
+  assumes "P \<leadsto>[(X O p2rel (~))] Q" 
+    and p: "Q ~ Q'" 
+  shows "P \<leadsto>[(X O p2rel (~))] Q'"
+proof -
+  let ?Y = "X O p2rel (~)"
+  show ?thesis
+  proof -
+    have "?Y O (p2rel (~)) \<subseteq> ?Y" using bisim_trans by fastforce
+    then show ?thesis 
+      using assms by (smt (verit, ccfv_threshold) basic_trans_rules(24) bisim.simps bisim_refl in_p2_rel_simp relcomp.intros sim_def sim_set_def subrelI)
+  qed
+qed
+
+lemma simWeakSim:
+  assumes "P \<leadsto>[Rel] Q"
+  shows "P \<leadsto>\<^sup>^<Rel> Q"
+using assms
+  apply(rule_tac weakSimI, auto)
+  apply (meson sim_set_def step_wstep)
+  done
+
+lemma wsim_set_bisim_r:
+  assumes "P \<leadsto>[(X O p2rel (~))] Q" 
+    and p: "Q ~ Q'" 
+  shows "P \<leadsto>\<^sup>^<(X O p2rel (\<approx>))> Q'"
+  using assms apply -
+  apply (rule simWeakSim)
+  apply (drule sim_set_bisim_r)
+   apply assumption
+  apply (smt (verit, ccfv_threshold) bisim_wbisim in_p2_rel_simp relcomp.simps sim_set_def) 
+  done
+
+
+lemma wsim_set_bisim_l:
+  assumes "P' \<leadsto>\<^sup>^<(p2rel (~) O X)> Q" 
+    and p: "P ~ P'" 
+  shows "P \<leadsto>\<^sup>^<(p2rel (~) O X)> Q"
+proof -
+  let ?Y = "p2rel (~) O X"
+  show ?thesis
+  proof -
+    have "(p2rel (~)) O ?Y \<subseteq> ?Y" using bisim_trans by fastforce
+    then show ?thesis 
+      using assms apply -
+      apply (rule wsimTransitive)
+         prefer 3
+         apply assumption
+      apply simp_all
+      apply (metis bisim.cases bisim_converse simWeakSim sim_set_sim)
+      done
+  qed
+qed
+
+lemma wbisim_absorb_bisim_l:
+  "(X O p2rel (~)) O p2rel (\<approx>) \<subseteq> X O p2rel (\<approx>)"
+  by (smt (verit) bisim_wbisim in_p2_rel_simp relcomp.simps relcompE subset_iff wbisim_trans)
+
+
+lemma wbisim_absorb_bisim_r:
+  "X O p2rel (\<approx>) O p2rel (~) \<subseteq> X O p2rel (\<approx>)"
+  by (smt (verit) bisim_wbisim in_p2_rel_simp relcomp.simps relcompE subset_iff wbisim_trans)
+
+lemma
+  "(P', Q') \<in> p2rel (\<approx>) O X O p2rel (~) \<Longrightarrow> Q' \<leadsto>\<^sup>^<p2rel (\<approx>)> Q \<Longrightarrow> P' \<leadsto>\<^sup>^<(p2rel (\<approx>) O X O p2rel (\<approx>))> Q"
+  oops
+
+lemma wbisim_wsim_setD:
+  "Q' \<approx> Q \<Longrightarrow> Q' \<leadsto>\<^sup>^<(p2rel (\<approx>))> Q \<and> Q \<leadsto>\<^sup>^<(p2rel (\<approx>))> Q'"
+  by (simp add: wbisim.simps wsim_set_wsim)
+
+lemma wsim_set_wbisim_bisim_r_l:
+  assumes sim: "P' \<leadsto>\<^sup>^<(p2rel (\<approx>) O X O p2rel (~))> Q'"
+    and Q: "Q' ~ Q"
+    and P: "P \<approx> P'"
+  shows "P \<leadsto>\<^sup>^<(p2rel (\<approx>) O X O p2rel (~))> Q"
+  using assms proof -
+  let ?Y = "p2rel (\<approx>) O X O p2rel (~)"
+  show ?thesis
+  proof -
+    note Q
+    then have qsim: "Q' \<leadsto>[p2rel (~)] Q" by (simp add: bisim.simps sim_set_sim)
+    moreover have "?Y O p2rel (~) \<subseteq> ?Y" by (smt (z3) O_assoc bisim_trans in_p2_rel_simp relcomp.inducts relcomp_mono subrelI)
+    ultimately
+    have "P' \<leadsto>\<^sup>^<?Y> Q"
+      apply -
+      apply (rule strongAppend)
+        apply (rule sim)
+       apply assumption+
+      done
+    moreover note \<open>P \<approx> P'\<close>
+    moreover have "(p2rel (\<approx>)) O ?Y \<subseteq> ?Y" using wbisim_trans by fastforce
+    ultimately have "P \<leadsto>\<^sup>^<?Y> Q" 
+      apply -
+      apply (rule wsimTransitive)
+         prefer 3
+         apply assumption
+        apply simp_all
+      apply (metis wbisim.cases wbisim_converse wsim_set_wsim)+
+      done
+    then show ?thesis.
+  qed
+qed
+
+
+lemma wsim_set_bisim_wbisim_r_l:
+  assumes sim: "P' \<leadsto>\<^sup>^<(p2rel (~) O X O p2rel (\<approx>))> Q'"
+    and P: "P ~ P'"
+    and Q: "Q \<approx> Q'"
+  shows "P \<leadsto>\<^sup>^<(p2rel (~) O X O p2rel (\<approx>))> Q"
+  using assms apply -
+  apply (rule wsim_set_bisim_l[rotated])
+   apply assumption
+  oops
+
+lemma weakBisimWeakUpto_rSim_aux:
+  assumes eq1: "P \<approx> P'" 
+    and eq2: "Q' ~ Q"
+    and inn: "(P', Q') \<in> X" 
+    and rSim: "\<And>P Q. (P, Q) \<in> X \<Longrightarrow> P \<leadsto>\<^sup>^<((p2rel (\<approx>)) O X O (p2rel (~)))> Q"
+  shows "P \<leadsto>\<^sup>^<(p2rel (\<approx>) O X O p2rel (~))> Q"
+  using assms wsim_set_wbisim_bisim_r_l by blast
+
+
+lemma weakBisimWeakUpto_rSym_aux:
+  assumes eq1: "P ~ P'" 
+    and eq2: "Q' \<approx> Q"
+    and inn: "(P', Q') \<in> X" 
+    and rSym: "\<And>P Q. (P, Q) \<in> X \<Longrightarrow> Q \<leadsto>\<^sup>^<((p2rel (\<approx>)) O X O (p2rel (~)))> P"
+  shows "Q \<leadsto>\<^sup>^<(p2rel (\<approx>) O X O p2rel (~))> P"
+  using assms wsim_set_wbisim_bisim_r_l bisim_sym wbisim_sym by blast
+
+lemma weakBisimWeakUpto_rSim:
+  "(P', Q') \<in> p2rel (\<approx>) O X O p2rel (~) \<Longrightarrow>
+   Q' \<leadsto>\<^sup>^<p2rel (\<approx>)> Q \<Longrightarrow>
+   (\<And>P Q. (P, Q) \<in> X \<Longrightarrow> P \<leadsto>\<^sup>^<(p2rel (\<approx>) O X O p2rel (~))> Q) \<Longrightarrow>
+   P' \<leadsto>\<^sup>^<(p2rel (\<approx>) O X O p2rel (\<approx>))> Q"
+  apply (subgoal_tac "(p2rel (\<approx>) O X O p2rel (~)) O p2rel (\<approx>) \<subseteq> p2rel (\<approx>) O X O p2rel (\<approx>)")
+  apply (smt (verit, ccfv_threshold) in_p2_rel_simp relcomp.cases wsimTransitive wsim_set_wbisim_bisim_r_l)
+  using wbisim_absorb_bisim_l apply fastforce
+  done
+
+lemma weakBisimWeakUpto_rSim:
+  "(P', Q') \<in> p2rel (\<approx>) O X O p2rel (~) \<Longrightarrow>
+   P' \<leadsto>\<^sup>^<p2rel (\<approx>)> P \<Longrightarrow>
+   (\<And>P Q. (P, Q) \<in> X \<Longrightarrow> Q \<leadsto>\<^sup>^<((p2rel (\<approx>)) O X O (p2rel (~)))> P) \<Longrightarrow>
+   Q \<leadsto>\<^sup>^<(p2rel (\<approx>) O X O p2rel (\<approx>))> P'"
+  apply (subgoal_tac "(p2rel (\<approx>) O X O p2rel (~)) O p2rel (\<approx>) \<subseteq> p2rel (\<approx>) O X O p2rel (\<approx>)")
+  oops
+(* 
+  oops
+  apply (subgoal_tac "(p2rel (\<approx>) O X O p2rel (~)) O p2rel (\<approx>) \<subseteq> p2rel (\<approx>) O X O p2rel (\<approx>)")
+   apply (rule wsimTransitive)
+      prefer 3
+      apply assumption
+     apply simp_all
+  subgoal for S T
+    apply safe
+    apply simp
+    subgoal for P'' Q'' S' T'
+      apply (rule weakBisimWeakUpto_rSym_aux)
+      apply (subst bisim_sym)
+      apply assumption+
+      apply (subst wbisim_sym)
+      apply assumption+
+      apply simp_all *)
+
+
+lemma weakBisimWeakUpto_rSym:
+  assumes rSym: "(\<And>P Q. (P, Q) \<in> X \<Longrightarrow> Q \<leadsto>\<^sup>^<(p2rel (~) O X O p2rel (\<approx>))> P)"
+  shows
+  "(P', Q') \<in> p2rel (\<approx>) O X O p2rel (~) \<Longrightarrow>
+   Q \<leadsto>\<^sup>^<p2rel (\<approx>)> Q' \<Longrightarrow>
+   Q \<leadsto>\<^sup>^<(p2rel (\<approx>) O X O p2rel (\<approx>))> P'"
+  apply safe
+  apply simp
+   apply (rule wsimTransitive[of ])
+     prefer 2
+  apply (rule wsim_set_bisim_r)
+  oops
+
+lemma wsim_set_def_converse_wbisim_cong:
+  "P \<leadsto>\<^sup>^<converse X> Q \<Longrightarrow> P \<leadsto>\<^sup>^<p2rel (wbisim_cong (rel2p X))> Q"
+  unfolding wsim_set_def
+  apply safe
+  apply (metis converse.cases in_p2_rel_simp rel2p_def wbisim_cong.wbc_base wbisim_cong.wbc_sym)
+  done
+
+term symclp
+
+find_theorems symclp conversep
+
+lemma wsim_set_def_disjI:
+  "P \<leadsto>\<^sup>^<Y> Q \<or> P \<leadsto>\<^sup>^<X> Q \<Longrightarrow> P \<leadsto>\<^sup>^<(Y \<union> X)> Q"
+  unfolding wsim_set_def
+   apply blast
+  done
+
+lemma weakBisimWeakUpto[case_names cSim cSym, consumes 1]:
+  assumes p: "(P, Q) \<in> X"
+    and rSim: "\<And>P Q. (P, Q) \<in> X \<Longrightarrow> P \<leadsto>\<^sup>^<((p2rel (\<approx>)) O X O (p2rel (~)))> Q"
+    and rSym: "\<And> P Q. (P, Q) \<in> X \<Longrightarrow> Q \<leadsto>\<^sup>^<((p2rel (\<approx>)) O converse X O (p2rel (~)))> P"
+  shows "P \<approx> Q"
+proof -
+  let ?X = "p2rel (\<approx>) O X O p2rel (\<approx>)"
+  let ?Y = "p2rel (\<approx>) O X O p2rel (~)"
+  from \<open>(P, Q) \<in> X\<close> have "(P, Q) \<in> (?X \<union> converse ?X)" by (metis UnI1 in_p2_rel_simp relcomp.relcompI wbisim_refl)
+  thus ?thesis
+  proof(coinduct rule: weakBisimWeakCoinduct)
+    case(cSim P Q)
+    thus ?case 
+      apply safe
+       apply simp_all
+      subgoal for P' Q'
+        apply (frule wbisim_wsim_setD[of  P])
+        apply (frule wbisim_wsim_setD[of _ Q])
+        apply safe
+        apply (rule wsim_set_def_disjI)
+        apply (rule disjI1)
+        apply (rule weakBisimWeakUpto_rSim[rotated, OF _ rSim])
+          apply assumption+
+        apply (intro relcompI)
+          apply simp_all
+        apply (rule bisim_refl)
+        done
+      subgoal for Q' P'
+        apply (frule wbisim_wsim_setD[of  P'])
+        apply (frule wbisim_wsim_setD[of _ Q'])
+        apply safe
+        apply (rule wsim_set_def_disjI)
+        apply (rule disjI2)
+        apply (simp add: converse_relcomp O_assoc)
+        apply (rule weakBisimWeakUpto_rSim[rotated])
+          apply assumption+
+         defer
+         apply (intro relcompI)
+           apply simp_all
+        using wbisim_sym apply blast
+         apply (rule bisim_refl)
+        using rSym apply blast
+        done
+      done
+  next
+    case(cSym P Q)
+    thus ?case 
+      apply -
+      apply safe
+       apply simp_all
+      subgoal for P' Q'
+        apply (frule wbisim_wsim_setD[of  P])
+        apply (frule wbisim_wsim_setD[of _ Q])
+        apply safe
+        apply (rule wsim_set_def_disjI)
+        apply (simp add: converse_relcomp O_assoc)
+        apply (rule disjI2)
+        apply (rule weakBisimWeakUpto_rSim[rotated])
+          apply assumption+
+         defer
+         apply (intro relcompI)
+           apply simp_all
+        using wbisim_sym apply blast
+         apply (rule bisim_refl)
+        using rSym apply blast
+        done
+      subgoal for Q' P'
+        apply (frule wbisim_wsim_setD[of  P'])
+        apply (frule wbisim_wsim_setD[of _ Q'])
+        apply safe
+        apply (rule wsim_set_def_disjI)
+        apply (simp add: converse_relcomp O_assoc)
+        apply (rule disjI1)
+        apply (rule weakBisimWeakUpto_rSim[rotated])
+          apply assumption+
+         defer
+         apply (intro relcompI)
+           apply simp_all
+         apply (rule bisim_refl)
+        using rSim apply blast
+        done
+      done
+  qed
+qed
+
+lemma weakBisimUpto[case_names cSim cSym, consumes 1]:
+  assumes p: "(P, Q) \<in> X"
+  and rSim: "\<And>R S. (R, S) \<in> X \<Longrightarrow> R \<leadsto>\<^sup>^<(p2rel (\<approx>) O (X \<union> p2rel (\<approx>)) O p2rel (~))> S"
+  and rSym: "\<And>R S. (R, S) \<in> X \<Longrightarrow> S \<leadsto>\<^sup>^<(p2rel (\<approx>) O (converse X \<union> p2rel (\<approx>)) O p2rel (~))> R"
+  shows "P \<approx> Q"
+proof -
+  from p have "(P, Q) \<in> X \<union> p2rel (\<approx>)" by simp
+  thus ?thesis
+    apply(coinduct rule: weakBisimWeakUpto)
+     apply(auto dest: rSim rSym)
+    unfolding wsim_set_def
+      apply (metis (no_types, opaque_lifting) UnI1 bisim_refl in_p2_rel_simp inf_sup_aci(5) p2rel_relcompp relcomppI wbisim_refl wbisim_sym wbisim_wstep_alt)
+    apply (metis rSym converse_add_simps(3) p2rel_converse wbisim_converse weakSimE)
+    apply (smt (verit, ccfv_SIG) UnI2 bisim_refl converse_iff in_p2_rel_simp relcomp.relcompI wbisim_refl wbisim_wstep_alt)
+    done
+qed
+
+thm weakBisimWeakUpto[where X="p2rel R", unfolded wsim_set_wsim p2rel_relcompp, no_vars]
+
+lemma
+  "(P, Q) \<in> p2rel R \<Longrightarrow>
+(\<And>P Q. (P, Q) \<in> p2rel R \<Longrightarrow> P \<leadsto>\<^sup>^<(p2rel (\<approx>) O p2rel R O p2rel (~))> Q) \<Longrightarrow>
+(\<And>P Q. (P, Q) \<in> p2rel R \<Longrightarrow> Q \<leadsto>\<^sup>^<(p2rel (\<approx>) O (p2rel R)\<inverse> O p2rel (~))> P) \<Longrightarrow> P \<approx> Q"
+  apply (simp_all add: wsim_set_wsim flip: p2rel_relcompp)
+  apply (simp add: converse_relcompp relcompp_assoc)
+  oops
+
+  find_theorems " (_  OO _)" name: assoc
+
+lemma weakBisimWeakUptoBisim[case_names SIM1 SIM2, consumes 1]:
+  assumes p: "R op1 op2"
+  and rSim: "\<And>op1 op2. R op1 op2 \<Longrightarrow> wsim ((~) OO R OO (\<approx>)) op1 op2"
+   and rSym: "\<And>op1 op2. R op1 op2 \<Longrightarrow> wsim ((~) OO R\<inverse>\<inverse> OO (\<approx>)) op2 op1"
+ shows "op1 \<approx> op2"
+  apply (rule weakBisimWeakUpto[where X="p2rel R"])
+  using assms(1) apply fastforce
+  apply (simp_all add: wsim_set_wsim flip: p2rel_relcompp)
+  apply (simp_all add: converse_relcompp relcompp_assoc)
+   apply (rule rSym) 
+   apply assumption
+   apply (rule rSim) 
+  apply assumption
+  done
+
+lemma weakBisimWeakUptoBisim_alt[case_names SIM1 SIM2, consumes 1]:
+  assumes p: "R op1 op2"
+  and Sim: "\<And>op1 op2. R op1 op2 \<Longrightarrow> wsim ((~) OO R OO (\<approx>)) op1 op2 \<and> wsim ((~) OO R\<inverse>\<inverse> OO (\<approx>)) op2 op1"
+shows "op1 \<approx> op2"
+  using assms weakBisimWeakUptoBisim by metis
+
+term bisim_cong
+
+inductive wbisim_upto_bisim_cong ("\<U>") for R  where
+  wb_upto_b_base[intro]:  "R op1 op2 \<Longrightarrow> \<U> R op1 op2"
+| wb_upto_b_sym[intro]:  "\<U> R op2 op1 \<Longrightarrow> \<U> R op1 op2"
+| wb_upto_b_Write[intro]: "\<U> R op1 op2 \<Longrightarrow> \<U> R (Write op1 p x) (Write op2 p x)"
+| wb_upto_b_Sim:"sim (\<U> R) op1 op2 \<Longrightarrow> sim (\<U> R) op2 op1 \<Longrightarrow> \<U> R op1 op2"
+| wb_upto_b_writes[intro]: "\<U> R op1 op2 \<Longrightarrow> \<U> R (writes op1 p x) (writes op2 p x)"
+| wb_upto_b_Silent[intro]: "\<U> R op1 op2 \<Longrightarrow> \<U> R (Silent op1) (Silent op2)"
+
+term bisim_cong
+
+(* | wbc_bisim:  "wbisim x y \<Longrightarrow> wbisim_cong R x y"
+| wbc_refl[intro]: "x = y \<Longrightarrow> wbisim_cong R x y"
+| wbc_sym[intro]: "wbisim_cong R x y \<Longrightarrow> wbisim_cong R y x"
+| wbc_Read:"x1 = y1 \<Longrightarrow> rel_fun (=) (wbisim_cong R) x2 y2 \<Longrightarrow> wbisim_cong R (Read x1 x2) (Read y1 y2)"
+| wbc_Write: "wbisim_cong R x1 y1 \<Longrightarrow> wbisim_cong R (Write x1 x2 x3) (Write y1 x2 x3)"
+| wbc_Silent: "wbisim_cong R x1 y1 \<Longrightarrow> wbisim_cong R (Silent x1) (Silent y1)"
+lemma lambda_disj_conversep[simp]:
+  "(\<lambda>a b. R a b \<or> a \<approx> b)\<inverse>\<inverse> = (\<lambda>a b. R b a \<or> a \<approx> b)" *)
+
+
+lemma weakBisimWeakUptoBisimCong[case_names SIM1 SIM2, consumes 1]:
+  assumes p: "R op1 op2"
+  and rSim: "\<And>op1 op2. R op1 op2 \<Longrightarrow> wsim (((~) OO \<U> R OO (\<approx>))) op1 op2"
+   and rSym: "\<And>op1 op2. R op1 op2 \<Longrightarrow> wsim (((~) OO \<U> R OO (\<approx>))) op2 op1"
+ shows "op1 \<approx> op2"
+  using assms apply -
+  apply (rule weakBisimWeakUptoBisim_alt[where R="\<U> R", of op1 op2])
+  subgoal
+    apply (rule wb_upto_b_base)
+    apply auto
+    done
+  subgoal premises prems for s' t'
+    using prems(4-) apply -
+    apply (induct s' t' pred: wbisim_upto_bisim_cong)
+    subgoal for x y
+      apply (intro conjI)
+      using prems(2) apply blast
+      using prems(3) apply (metis (no_types, opaque_lifting) conversep_iff order_antisym_conv predicate2I_obj wbisim_upto_bisim_cong.intros(2))
+      done
+    subgoal for x y
+      apply (intro conjI)
+      apply (metis conversepD conversep_le_swap order_antisym_conv predicate2I_obj wbisim_upto_bisim_cong.intros(2))+
+      done
+    subgoal for op1 op2 p x
+      apply (intro conjI)
+       apply (metis (no_types, opaque_lifting) OO_def bisim_refl step.intros(2) step_wstep wbisim_refl wsim_Write)
+      apply clarsimp
+      using prems(2,3)
+      apply (metis (no_types, lifting) SW bisim_refl relcompp_apply step_wstep wbisim_refl)
+      done
+    subgoal for op1s op2s
+      apply (intro conjI)
+      subgoal
+        unfolding wsim_def sim_def
+        apply (auto simp del: cin.rep_eq)
+        apply (metis bisim_refl relcompp_apply step_wstep wbisim_refl_alt)
+        done
+      subgoal
+        unfolding wsim_def sim_def
+        apply (auto simp del: cin.rep_eq)
+        apply (metis bisim_refl conversep_iff relcompp_apply step_wstep wbisim_refl wbisim_upto_bisim_cong.intros(2))
+        done
+      done
+    subgoal sorry
+    subgoal sorry
+    done
+  done
+
+
+(* FIXME: move me *)
+lemma steps_writes:
+  "ios = map (Out p) xs \<Longrightarrow>
+   steps ios (writes op p xs) op"
+  apply (induct ios arbitrary: xs)
+   apply (force simp add: writes_Cons_simp)+
+  done
+
+lemma cfilter_eq_forall_eq:
+  "cfilter F C = cfilter F C' \<longleftrightarrow>
+   (\<forall> c. F c \<longrightarrow> c |\<in>| C \<longleftrightarrow> c |\<in>| C')"
+  by auto
+
+lemma map_op_writes[simp]:
+  "map_op f1 f2 (writes op p xs) = writes (map_op f1 f2 op) (f2 p) xs"
+  apply (induct xs)
+   apply (simp_all add: writes_Cons_simp)
+  done
+
+
+
+
+(* find_theorems nd_writes
+
+friend_of_corec nd_writes where
+  "nd_writes op p xs =
+    (case op of 
+     Read p' f \<Rightarrow> Read p' (\<lambda> x'. nd_writes (f x') p xs)
+   | Write op' p' x' \<Rightarrow> (if p = p' then Write (nd_writes op' p (tl (xs @ [x']))) p (hd (xs @ [x'])) else Write (nd_writes op' p xs) p' x')
+   | Choice ops \<Rightarrow> Choice (cimage (\<lambda> op. nd_writes op p xs) ops)
+   | Silent op' \<Rightarrow> Silent (nd_writes op' p xs))"
+   apply (rule nd_writes.code)
+  apply transfer_prover
+  done
+ *)
+ 
+
+
+(* 
+friend_of_corec nd_writes where
+"nd_writes op p xs =
+   Choice (cimage (\<lambda> op. case op of
+   Write op' p' x' \<Rightarrow> (if p = p' then let xs' = xs @ [x'] in Write (nd_writes op' p (tl xs')) p (hd xs') else Write (nd_writes op' p xs) p' x')
+ | Silent op' \<Rightarrow> Silent (nd_writes op' p xs)
+ | Read p' f \<Rightarrow> Read p' (\<lambda> x'. nd_writes (f x') p xs)
+ )
+ (choices op))" 
+*)
+
+lemma step_nd_writes_elim:                  
+  assumes "step io (nd_writes op p xs) op'"
+  obtains 
+    x x' xs' op'' where "io = Out p x" "xs @ [x'] = x # xs'" "op' = nd_writes op'' p xs'" "step (Out p x') op op''"
+  | p' x' op'' where "io = Out p' x'" "op' = nd_writes op'' p xs" "step (Out p' x') op op''"
+  | p' x' op'' where "io = Inp p' x'" "op' = nd_writes op'' p xs" "step (Inp p' x') op op''"
+  | op'' where "io = Tau" "op' = nd_writes op'' p xs" "step Tau op op''"
+ (*  using assms apply atomize_elim
+  apply (induct "nd_writes op p xs" op' arbitrary: op pred: step)
+  subgoal
+    apply (subst (asm) nd_writes.code)
+    apply (clarsimp simp flip: cin.rep_eq del: disjCI split: op.splits if_splits; force)
+    done
+  subgoal
+    apply (cases xs)
+    subgoal
+    apply (subst (asm) nd_writes.code)
+    apply (auto simp flip: cin.rep_eq del: disjCI split: op.splits if_splits)
+    done
+    subgoal
+    apply (subst (asm) nd_writes.code)
+    apply (auto simp flip: cin.rep_eq del: disjCI split: op.splits if_splits)
+      apply force+
+      done
+    done
+  subgoal
+    apply (subst (asm) nd_writes.code)
+    apply (clarsimp simp flip: cin.rep_eq del: disjCI split: op.splits if_splits; force)
+    done
+  subgoal for op' ops io op'' op'''
+    apply (clarsimp simp flip: cin.rep_eq del: disjCI split: if_splits)
+    apply (subst (asm) (6) nd_writes.code)
+    apply (clarsimp simp flip: cin.rep_eq del: disjCI split: op.splits if_splits; hypsubst_thin)
+    apply (drule meta_spec)
+    apply (drule meta_mp)
+     apply simp
+    apply (smt (verit, ccfv_threshold) step.intros(4))
+    done
+  done *)
+  oops
 
 end
